template-coq/src/constr_quoter.ml
@@ -302,8 +302,7 @@ struct
     let const' = quote_univ_constraints (UContext.constraints (AbstractContext.repr uctx)) in
     constr_mkApp (tAUContextmake, [|idents; const'|])
 
-  let mkMonomorphic_ctx t =
-    constr_mkApp (cMonomorphic_ctx, [|t|])
+  let mkMonomorphic_ctx () = Lazy.force cMonomorphic_ctx
 
   let mkPolymorphic_ctx t =
     constr_mkApp (cPolymorphic_ctx, [|t|])
@@ -411,6 +410,9 @@ struct
   let add_global_decl kn d l =
     let pair = pairl tkername tglobal_decl kn d in
     constr_mkApp (c_cons, [| global_pairty (); pair; l|])
+
+  let mk_global_env univs decls =
+    constr_mkApp (tBuild_global_env, [| univs; decls |])
 
   let mk_program f s = pairl tglobal_env tTerm f s
 
