template-coq/src/quoter.ml
@@ -101,7 +101,7 @@ sig
   val mkMonomorphic_entry : quoted_univ_contextset -> quoted_universes_entry
   val mkPolymorphic_entry : quoted_univ_context -> quoted_universes_entry
 
-  val mkMonomorphic_ctx : quoted_univ_contextset -> quoted_universes_decl
+  val mkMonomorphic_ctx : unit -> quoted_universes_decl
   val mkPolymorphic_ctx : quoted_abstract_univ_context -> quoted_universes_decl
 
   val quote_mind_finiteness : Declarations.recursivity_kind -> quoted_mind_finiteness
@@ -148,9 +148,10 @@ sig
 
   val mk_constant_decl : quoted_constant_body -> quoted_global_decl
 
-  val empty_global_declarations : unit -> quoted_global_env
-  val add_global_decl : quoted_kernel_name -> quoted_global_decl -> quoted_global_env -> quoted_global_env
-
+  val empty_global_declarations : unit -> quoted_global_declarations
+  val add_global_decl : quoted_kernel_name -> quoted_global_decl -> quoted_global_declarations -> quoted_global_declarations
+  
+  val mk_global_env : quoted_univ_contextset -> quoted_global_declarations -> quoted_global_env
   val mk_program : quoted_global_env -> t -> quoted_program
 end
 
@@ -173,13 +174,31 @@ struct
 
   let quote_universes_decl decl templ =
     match decl with
-    | Monomorphic -> 
-      (* (match templ with
-      | Some { template_context = ctx } ->
-        Q.mkMonomorphic_ctx (Q.quote_univ_contextset ctx)
-      | None -> *)
-        Q.mkMonomorphic_ctx (Q.quote_univ_contextset Univ.ContextSet.empty)
+    | Monomorphic -> Q.mkMonomorphic_ctx ()
     | Polymorphic ctx -> Q.mkPolymorphic_ctx (Q.quote_abstract_univ_context ctx)
+
+  let quote_ugraph ?kept (g : UGraph.t) =
+    let levels, cstrs, eqs = 
+      match kept with
+      | None ->
+        let cstrs, eqs = UGraph.constraints_of_universes g in
+        UGraph.domain g, cstrs, eqs
+      | Some l ->
+        let cstrs = UGraph.constraints_for ~kept:l g in
+        l, cstrs, []
+    in
+    let levels, cstrs = 
+      List.fold_right (fun eqs acc ->
+        match Univ.Level.Set.elements eqs with
+        | [] -> acc
+        | x :: [] -> acc
+        | x :: rest ->
+          List.fold_right (fun p (levels, cstrs) ->
+            (Univ.Level.Set.add p levels, Univ.Constraints.add (x, Univ.Eq, p) cstrs)) rest acc)
+        eqs (levels, cstrs)
+    in
+    let levels = Univ.Level.Set.remove Univ.Level.set levels in
+    Q.quote_univ_contextset (levels, cstrs)
 
   let quote_inductive' (ind, i) : Q.quoted_inductive =
     Q.quote_inductive (Q.quote_kn (Names.MutInd.canonical ind), Q.quote_int i)
@@ -413,9 +432,26 @@ struct
     Ind of Names.inductive * mutual_inductive_body
   | Const of KerName.t
 
+  let universes_of_ctx ctx = 
+    Context.Rel.fold_inside (fun univs d -> Univ.Level.Set.union univs
+      (Context.Rel.Declaration.fold_constr (fun c univs -> Univ.Level.Set.union univs (Vars.universes_of_constr c)) d univs))
+      ~init:Univ.Level.Set.empty ctx
+  
+  let universes_of_mib mib = 
+    let pars = mib.mind_params_ctxt in
+    let univs = universes_of_ctx pars in
+      Array.fold_left (fun univs oib ->
+        let univsty = universes_of_ctx oib.mind_arity_ctxt in
+        Array.fold_left (fun univs cty -> 
+          let univscty = Vars.universes_of_constr cty in
+          Univ.Level.Set.union univs univscty)
+          univsty oib.mind_user_lc)
+        univs mib.mind_packets
+
   let quote_term_rec bypass env trm =
     let visited_terms = ref Names.KNset.empty in
     let visited_types = ref Mindset.empty in
+    let universes = ref Univ.Level.Set.empty in
     let constants = ref [] in
     let add quote_term quote_type trm acc =
       match trm with
@@ -424,7 +460,9 @@ struct
         if Mindset.mem t !visited_types then ()
         else
           begin
-            visited_types := Mindset.add t !visited_types ;
+            visited_types := Mindset.add t !visited_types;
+            let univs = universes_of_mib mib in
+            let () = universes := Univ.Level.Set.union univs !universes in
             let (kn,d,acc) =
               try quote_type acc env mi mib
               with e ->
@@ -458,6 +496,8 @@ struct
               match body with
               | None -> None, acc
               | Some tm -> 
+                let univs = Vars.universes_of_constr tm in
+                let () = universes := Univ.Level.Set.union univs !universes in
                 try let (tm, acc) = quote_term acc (Global.env ()) tm in
                   (Some tm, acc)
                 with e ->
@@ -467,6 +507,8 @@ struct
             let uctx = quote_universes_decl cd.const_universes None in
             let ty, acc =
               let ty = cd.const_type in
+              let univs = Vars.universes_of_constr ty in
+              let () = universes := Univ.Level.Set.union univs !universes in
               (try quote_term acc (Global.env ()) ty
                 with e ->
                   Feedback.msg_debug (str"Exception raised while checking type of " ++ KerName.print kn);
@@ -488,9 +530,12 @@ struct
       b := y ;
       (x,y)
     in
+    let univs = Univ.Level.Set.union (Vars.universes_of_constr trm) !universes in
     let (tm, _) = quote_rem () env trm in
-    let decls =  List.fold_right (fun (kn, d) acc -> Q.add_global_decl kn d acc)  !constants (Q.empty_global_declarations ()) in
-    Q.mk_program decls tm
+    let decls = List.fold_right (fun (kn, d) acc -> Q.add_global_decl kn d acc)  !constants (Q.empty_global_declarations ()) in
+    let univs = quote_ugraph ~kept:univs (Environ.universes env) in
+    let env = Q.mk_global_env univs decls in
+    Q.mk_program env tm
 
   let quote_rel_context env ctx =
     fst (quote_rel_context (fun acc env t -> (quote_term (snd env) t, acc)) () ((), env) ctx)
@@ -582,7 +627,4 @@ since  [absrt_info] is a private type *)
   let quote_entry_of bypass env evm t =
     try Some (quote_entry_aux bypass env evm t)
     with Not_found -> None *)
-
-  let quote_ugraph (g : UGraph.t) =
-    Q.quote_univ_constraints (fst (UGraph.constraints_of_universes g))
 end
