template-coq/theories/AstUtils.v
@@ -191,7 +191,7 @@ Fixpoint lookup_mind_decl (id : kername) (decls : global_declarations)
 Definition universes_entry_of_decl (u : universes_decl) : universes_entry :=
   match u with
   | Polymorphic_ctx ctx => Polymorphic_entry (Universes.AUContext.repr ctx)
-  | Monomorphic_ctx ctx => Monomorphic_entry ctx
+  | Monomorphic_ctx => Monomorphic_entry ContextSet.empty
   end.
 
 (* TODO factorize in Environment *)
