template-coq/theories/Reflect.v
@@ -435,7 +435,7 @@ Proof.
   cong.
 Defined.
 
-(*Definition eqb_ConstraintSet x y :=
+Definition eqb_ConstraintSet x y :=
   eqb (ConstraintSet.this x) (ConstraintSet.this y).
 
 #[global] Instance reflect_ConstraintSet : ReflectEq ConstraintSet.t.
@@ -447,9 +447,9 @@ Proof.
   destruct (eqb_spec thisx thisy); subst; constructor.
   - f_equal; apply uip.
   - congruence.
-Defined.*)
+Defined.
 
-(*Definition eqb_LevelSet x y :=
+Definition eqb_LevelSet x y :=
   eqb (LevelSet.this x) (LevelSet.this y).
 
 #[global] Instance reflect_LevelSet : ReflectEq LevelSet.t.
@@ -461,7 +461,7 @@ Proof.
   destruct (eqb_spec thisx thisy); subst; constructor.
   - f_equal; apply uip.
   - congruence.
-Defined.*)
+Defined.
 
 Ltac finish_reflect :=
   (repeat
@@ -470,9 +470,9 @@ Ltac finish_reflect :=
     end);
   constructor; trivial; congruence.
 
-(*Definition eqb_universes_decl x y :=
+Definition eqb_universes_decl x y :=
   match x, y with
-  | Monomorphic_ctx cx, Monomorphic_ctx cy => eqb cx cy
+  | Monomorphic_ctx, Monomorphic_ctx => true
   | Polymorphic_ctx cx, Polymorphic_ctx cy => eqb cx cy
   | _, _ => false
   end.
@@ -484,7 +484,7 @@ Proof.
   unfold eqb_universes_decl.
   intros [] []; finish_reflect.
 Defined.
-*)
+
 Definition eqb_allowed_eliminations x y :=
   match x, y with
   | IntoSProp, IntoSProp
